theories/typing.v
@@ -1,21 +1,32 @@
 From iris.heap_lang Require Export lang.
+Require Import FunctionalExtensionality.
 
-Section typing.
+Inductive side : Set :=
+| Left
+| Right.
 
-  Inductive side : Set :=
-  | Left
-  | Right.
+Inductive stype :=
+| TEnd
+| TSend (P : val → Prop) (st : val → stype)
+| TRecv (P : val → Prop) (st : val → stype).
 
-  Inductive stype :=
-  | TEnd
-  | TSend (P : val → Prop) (sτ : val → stype)
-  | TRecv (P : val → Prop) (sτ : val → stype).
+Instance stype_inhabited : Inhabited stype := populate TEnd.
 
-  Fixpoint dual_stype (sτ :stype) :=
-    match sτ with
-    | TEnd => TEnd
-    | TSend P sτ => TRecv P (λ v, dual_stype (sτ v))
-    | TRecv P sτ => TSend P (λ v, dual_stype (sτ v))
-    end.
+Fixpoint dual_stype (st :stype) :=
+  match st with
+  | TEnd => TEnd
+  | TSend P st => TRecv P (λ v, dual_stype (st v))
+  | TRecv P st => TSend P (λ v, dual_stype (st v))
+  end.
 
-End typing.
+Class Involutive {T} (f : T → T) :=
+  involutive : ∀ t : T, t = f (f t).
+
+Instance dual_stype_involutive : Involutive dual_stype.
+Proof.
+  intros st.
+  induction st => //; simpl;
+    assert (st = (λ v : val, dual_stype (dual_stype (st v)))) as Heq
+        by apply functional_extensionality => //;
+    rewrite -Heq => //.
+Qed.
